Semantic/CoreCapybara/Denotation.lean
@@ -1,3 +1,4 @@
 import Semantic.CoreCapybara.Denotation.Core
 import Semantic.CoreCapybara.Denotation.Rebind
 import Semantic.CoreCapybara.Denotation.Retype
+import Semantic.CoreCapybara.Denotation.Kill
